incr/IncrA.v
@@ -5,30 +5,24 @@ Require Import MemHeader MemA.
 Require Import IncrHeader.
 
 Module IncrA. Section IncrA.
-  Context `{!crisG Γ Σ α β τ _S _I, !memGS, !concGS}.
+  Context `{!crisG Γ Σ α β τ Hsub Hinv, !memGS, !schGS}.
 
   Definition scopes : list string := [].
 
-  Definition incr_spec : fspec_atomic := {|
-    meta_priv := mblock * ptrofs;
-    meta_pub := Z;
-    pre_priv := λ bofs arg, ⌜arg = [Vptr bofs]↑⌝;
-    pre_pub := λ bofs v _, bofs ↦ Vint v;
-    post_pub := λ bofs v ret, bofs ↦ Vint (v + 1);
-    post_priv := λ bofs v ret, ⌜ret = (Vint v)↑⌝;
-  |}%I.
+  Definition incr (N : namespace) : fbody := λ arg,
+    {{{ ∀∀ bofs, ⌜arg = [Vptr bofs]↑⌝ }}}
+      <<{ ∀∀ v, bofs ↦ Vint v, bofs ↦ Vint (v + 1) }>>
+    {{{ ∀∀ v, RET ret, ⌜ret = (Vint v)↑⌝ }}} @ N.
 
-  Definition fnsems : fnsemmap :=
-    {[fid IncrHdr.incr #
-        (msk_scp scopes msk_true,
-          (None, atomic_fun incr_spec (atomic_update incr_spec)))]}.
+  Definition fnsems (N : namespace) : fnsemmap :=
+    {[fid IncrHdr.incr # (msk_scp scopes msk_true, (None, incr N))]}.
 
-  Program Definition smod : SMod.t := {|
+  Program Definition smod N : SMod.t := {|
     SMod.scopes := scopes;
-    SMod.fnsems := fnsems;
+    SMod.fnsems := fnsems N;
     SMod.initial_st := ∅;
   |}.
   Solve All Obligations with mod_tac.
 
-  Definition t : Mod.t := SMod.to_mod ∅ smod.
+  Definition t N : Mod.t := SMod.to_mod (SchA.sp ∅ (↑N)) (smod N).
 End IncrA. End IncrA.
