elimination_stack/StackIAPop.v
@@ -14,7 +14,7 @@ Section StackIM.
 
   (* Stack module being masked for eliminating the helping module *)
   Context (N : namespace) (sp sp_user : specmap).
-  
+
   Definition init_cond : iProp Σ := helping_auth 1 ∅%I.
 
   Local Notation MemA := (CFilter.filter (Helping.exports mn) (MemA.t sp)).
@@ -24,20 +24,18 @@ Section StackIM.
   Local Notation StackM := ((StackM.t mn N (SchA.sp ∅ (↑N)) ★ HelpingOn) ★ MemA ★ SchI).
   Local Notation StackI := ((CFilter.filter (Helping.exports mn) StackI.t ★ HelpingDummy) ★ MemA ★ SchI).
   Local Notation IstFull := (IstProd (IstSB [mn] (IstHelp mn)) IstEq).
-                                    
+
   Lemma pop_simF : ISim.sim_fun open StackM StackI IstFull (fid StackHdr.pop).
   Proof using.
-    cStartFunSim. rewrite /StackI.pop /StackM.pop.
-    rewrite /StackM.pop /atomic_body.
-    cStepsS. destruct _q as [[stid mtid] [[n vs] γs]].
-    iDestruct "ASM" as "[TID [_ [-> #[%stackb [%stackofs [-> Hinv]]]]]]". cStepsT.
+    cStartFunSim. rewrite /StackI.pop /StackM.pop /yield_iter. cStepsS; cStepsT.
+    aStepS. iIntros (mtid stid γs) "TID [%v [-> [%n #Hstack]]]".
+    iDestruct "Hstack" as "#[%stackb [%stackofs [-> Hinv]]]". cStepsT. cStepsS.
 
     (* Coinduction starts here *)
     iApply wsim_reset.
     cCoind CIH g' __ with st_src st_tgt. iIntros "[#Hinv [IST TID]] /=".
-    unfoldIterT. rewrite {1}/StackI._pop. cStepsT.
-    sYieldIR "IST" "TID". { case_bool_decide; set_solver. }
-    sYieldIR "IST" "TID". { case_bool_decide; set_solver. }
+    aUnfoldT. rewrite {1}/StackI._pop. cStepsT.
+    sYieldIR "IST" "TID". sYieldIR "IST" "TID".
 
     (* Stack load *)
     iInv "Hinv" as "[[%stack_rep [%offer_rep [%l [Hs [H↦ [Hlist Hoffer]]]]]]|[% ●]]" "close";
@@ -45,22 +43,21 @@ Section StackIM.
     { iExFalso. iDestruct "IST" as "[% [% [% [% [% [[% [% [IST ●2]]] ?]]]]]]".
       iCombine "●" "●2" gives %[WF _]%gmap_view_auth_dfrac_op_valid. ss.
     }
-
     mLoadT "H↦".
 
     destruct (decide (stack_rep = Vint 0%Z)); subst.
     { (* Empty stack - terminate *)
-      sYieldS. cStepsS. cForceS false. cStepsS.
+      sYieldS. cForceS false. cStepsS. aUnfoldS; sYieldS. cStepsS.
 
       (* Atomic update *)
       iCombine "Hs ASM" gives %[->%Excl_included%leibniz_equiv _]%auth_both_valid_discrete.
       destruct l; [|ss; iPoseProof "Hlist" as "[% [% [% [% [% [% ?]]]]]]"; clarify].
-      cForceS. iFrame. cStepsS.
+      cForceS (inr _). cForcesS. iFrame.
 
       iMod ("close" with "[Hs Hlist Hoffer H↦]") as "_".
       { iLeft. iFrame. }
-      sYieldIR "IST" "TID". { case_bool_decide; set_solver. }
-      sYieldS. cForceS. iFrame. iSplit; eauto. cStep. iSplit; done.
+      sYieldIR "IST" "TID".
+      sYieldS. cStep; iFrame. iModIntro; iSplit; ss.
     }
     (* Stack nonempty *)
     iPoseProof (list_inv_comparable with "Hlist") as "[Hlist [Hval #Hcomp]]".
@@ -71,11 +68,8 @@ Section StackIM.
     iMod ("close" with "[Hs Hlist H↦ ↦v ↦next2 Hoffer]") as "_".
     { iLeft. iFrame. iExists _, _, _, _; iFrame; eauto. }
 
-    sYieldIR "IST" "TID". { case_bool_decide; set_solver. }
-    sYieldIR "IST" "TID". { case_bool_decide; set_solver. }
-
-    mLoadT "↦next".
-    sYieldIR "IST" "TID". { case_bool_decide; set_solver. }
+    sYieldIR "IST" "TID". sYieldIR "IST" "TID".
+    mLoadT "↦next". sYieldIR "IST" "TID".
 
     iInv "Hinv" as "[[%stack_rep' [%offer_rep' [%l' [Hs [H↦ [Hlist Hoffer]]]]]]|[% ●]]" "close";
       cycle 1.
@@ -92,38 +86,37 @@ Section StackIM.
     iIntros "H↦ [Hval Hval2]". iClear "Hcomp". cStepsT.
     case_bool_decide; subst.
     { (* Pop success *)
-      sYieldS. cStepsS. cForceS false. cStepsS.
+      sYieldS. cForceS false. cStepS. aUnfoldS. sYieldS. cStepsS.
       destruct (stack_rep') as [[| |]|[bold ofsold]|]; inv Hcomp; case_bool_decide; ss.
-      destruct l'; ss.
+      destruct l'.
       { iPoseProof "Hlist" as "%"; ss. }
       iDestruct "Hlist" as "[% [% [% [% [% [% [Hpt1 [Hpt2 Hlist]]]]]]]]". des; clarify.
       iPoseProof (mem_points_to_singleton_agree with "↦next Hpt2") as "<-".
       iCombine "Hs ASM" gives %[->%Excl_included%leibniz_equiv _]%auth_both_valid_discrete.
       iMod (own_update_2 with "Hs ASM") as "[Hs ASM]".
       { eapply auth_update, option_local_update, (exclusive_local_update _ (Excl _)). done. }
-      cForceS; iFrame. cStepsS.
+      cForceS (inr _). cForcesS. iFrame.
       iMod ("close" with "[Hs Hlist H↦ Hoffer]") as "_".
       { iLeft. iFrame. }
-      sYieldIR "IST" "TID". { case_bool_decide; set_solver. }
+      sYieldIR "IST" "TID".
 
       iCombine "Hval Hval2" as "Hval".
-      iApply (wsim_mem_cmp with "Hval");
-        [try prove_inline_cond|try prove_sb_cond|ss|..]; eauto.
+      iApply (wsim_mem_cmp with "Hval"); [try prove_inline_cond|try prove_sb_cond|ss|..]; eauto.
       { case_bool_decide; ss; exfalso; naive_solver. }
       { iIntros "[[% [% $]] [% [% $]]] !> [$ $] //". }
       iIntros "[[% [% Hval]] _]". cStepsT.
-      sYieldIR "IST" "TID". { case_bool_decide; set_solver. }
+      sYieldIR "IST" "TID".
 
       mLoadT "Hval".
       iPoseProof (mem_points_to_singleton_agree with "Hval Hpt1") as "<-".
-      sYieldIR "IST" "TID". { case_bool_decide; set_solver. }
-      sYieldS. cForceS. iFrame. iSplit; eauto. cStep. iFrame. eauto.
+      sYieldIR "IST" "TID".
+      sYieldS. cStep; iFrame. iModIntro; iSplit; ss.
     }
 
     (* Pop failure *)
     iMod ("close" with "[↦next Hs Hoffer Hlist H↦]") as "_".
     { iLeft. iFrame. }
-    sYieldIR "IST" "TID". { case_bool_decide; set_solver. } cStepsT.
+    sYieldIR "IST" "TID". cStepsT.
     iCombine "Hval Hval2" as "Hval".
     iApply (wsim_mem_cmp with "Hval");
       [try prove_inline_cond|try prove_sb_cond|unfold_cris_defs|..]; eauto.
@@ -132,7 +125,7 @@ Section StackIM.
     assert (succ = 0%Z); last subst succ.
     { destruct stack_rep' as [[|?|?]|[? ?]|]; inv Hcomp; ss; case_bool_decide; des; clarify; ss. }
     cStepsT.
-    sYieldIR "IST" "TID". { case_bool_decide; set_solver. }
+    sYieldIR "IST" "TID".
 
     (* Check the offer *)
     clear dependent stack_rep' offer_rep offer_rep' l  l'.
@@ -144,19 +137,18 @@ Section StackIM.
     iDestruct "Hoffer" as "[↦offer Hoffer]".
     mLoadT "↦offer".
     rewrite /syn_is_offer; destruct (offer_rep) as [[|?|?]|[offerb offerofs]|]; solve_base_sl_red;
-      try iPoseProof ("Hoffer") as "%"; ss.
-    { cStepsT.
-      iMod ("close" with "[Hs H↦ Hlist ↦offer]") as "_".
+      try iPoseProof ("Hoffer") as "%".
+    { cStepsT. iMod ("close" with "[Hs H↦ Hlist ↦offer]") as "_".
       { iLeft; iFrame. solve_base_sl_red. }
       cByCoind CIH. iFrame. done.
     }
-    iDestruct "Hoffer" as (γo [[stid' mtid'] [[[n' s'] v'] γs']] reqid) "[OfferInv <-]".
+    iDestruct "Hoffer" as (γo [v' γs'] reqid) "[OfferInv <-]".
     iPoseProof ("OfferInv") as "#OfferInv".
 
     cStepsT.
     iMod ("close" with "[Hs H↦ Hlist ↦offer]") as "_".
     { iLeft; iFrame. solve_base_sl_red. repeat iExists _; iSplit; eauto. }
-    sYieldIR "IST" "TID". { case_bool_decide; set_solver. }
+    sYieldIR "IST" "TID".
 
     (* Try to take the offer *)
     iInv "OfferInv" as "[%offerst [↦offerst offer]] /=" "close".
@@ -172,24 +164,19 @@ Section StackIM.
 
       (* Help *)
       sYieldS. cForceS true. cStepsS.
-      rewrite {3}/SchA.sp; simpl_map.
       cInlineS. cStepsS.
       iDestruct "IST" as "[% [% [% [% [[-> ->] [[% [% [[-> ->] ●Help]]] IST]]]]]]".
       iPoseProof (helping_auth_token with "●Help offer") as "%Hreq".
       iMod (helping_auth_commit with "●Help offer") as "[●offer #◯offer]".
       iMod ("close" with "[offer↦ ◯offer]") as "_".
       { iExists 1; iFrame; case_decide; ss. }
-      rewrite /HelpingOn.help. cForceS reqid. cStepsS.
-      assert (Hsp : (SchA.sp ∅ (↑N)).1 !! fid SchHdr.yield = fsp_some (SchA.yield_spec (↑N))).
-      { rewrite /SchA.sp; simpl_map; ss. }
-      rewrite !Hsp.
-      cForceS (stid, mtid, tt). cForcesS. iFrame. iSplit; eauto. cStepsS.
+      rewrite /HelpingOn.help. simpl_map. cForceS reqid.
+      cForceS (stid, mtid, tt). cForcesS. iFrame. iSplit; first eauto. cStepsS.
       destruct _q as [[stid1 mtid1] []]. iDestruct "ASM" as "[TID [_ ->]]".
 
       (* Helpee's Atomic Assume *)
-      rewrite /HelpingOn.try_run. cStepsS. rewrite Hreq /=.
-      cStepsS.
-      clear dependent stack_rep offer_rep l.
+      rewrite /HelpingOn.try_run. cStepsS. rewrite Hreq /= /StackM.jobCode.
+      cStepsS. clear dependent stack_rep offer_rep l.
       iInv "Hinv" as "[[%stack_rep [%offer_rep [%l [Hs [H↦ [Hlist Hoffer]]]]]]|[% ●]]" "Close";
         cycle 1.
       { iExFalso. iCombine "●" "●offer" gives %[WF _]%gmap_view_auth_dfrac_op_valid. ss. }
@@ -198,18 +185,19 @@ Section StackIM.
       { eapply auth_update, option_local_update, (exclusive_local_update _ (Excl _)). done. }
 
       (* Helpee's Atomic Guarantee *)
-      cForceS; iFrame "Hl". cStepsS.
+      cForcesS; iFrame. cStepsS.
 
       (* My Atomic Assume *)
       iPoseProof (helping_auth_split (1/2) with "●offer") as "[●offer ●reclaim]"; ss.
       iMod ("Close" with "[●offer]") as "_".
       { iRight; iFrame. }
-      cForcesS. iFrame; iSplit; eauto. cStepsS.
+      cForcesS. iFrame; iSplit; eauto. cStepsS. aUnfoldS. sYieldS; cStepsS.
       iDestruct "ASM" as "[TID [_ ->]]".
       iCombine "Hs ASM'" gives %[->%Excl_included%leibniz_equiv _]%auth_both_valid_discrete. ss.
       iMod (own_update_2 with "Hs ASM'") as "[Hs Hl]".
       { eapply auth_update, option_local_update, (exclusive_local_update _ (Excl _)). done. }
-      cForceS; iFrame "Hl"; cStepsS.
+
+      cForceS (inr _). cForcesS. iFrame "Hl"; cStepsS.
       iInv "Hinv" as "[[% [% [% [Hs' _]]]]|[% ●]]" "close".
       { iExFalso. iCombine "Hs" "Hs'" gives %WF; inv WF. }
       iPoseProof ("●reclaim" with "●") as "●".
@@ -217,19 +205,18 @@ Section StackIM.
       { iLeft; iFrame. }
       iIst "IST" with "[● IST]".
       { iExists _, _, _, _; iFrame. iSplit; eauto. iPureIntro; esplits; eauto; set_solver. }
-      sYieldIR "IST" "TID". { case_bool_decide; set_solver. }
+      sYieldIR "IST" "TID".
 
       iAssert (emp)%I with "[]" as "E"; first done.
       iApply (wsim_mem_cmp with "E");
         [try prove_inline_cond|try prove_sb_cond|unfold_cris_defs|..]; eauto.
       iIntros "_". cStepsT.
-      sYieldIR "IST" "TID". { case_bool_decide; set_solver. }
-      sYieldIR "IST" "TID". { case_bool_decide; set_solver. }
+      sYieldIR "IST" "TID". sYieldIR "IST" "TID".
 
       (* Compare *)
       mLoadT "offerv".
-      sYieldIR "IST" "TID". { case_bool_decide; set_solver. }
-      sYieldS. cForcesS. iFrame. iSplit; eauto. cStep. iFrame. done.
+      sYieldIR "IST" "TID".
+      sYieldS. cStep; iFrame. iModIntro; iSplit; ss.
     }
 
     (* Failed to take the offer - repeat the whole process! *)
@@ -240,13 +227,13 @@ Section StackIM.
     iIntros "↦offerst _". cStepsT.
     iMod ("close" with "[↦offerst offer]") as "_".
     { iExists _; ss; iFrame. case_decide; clarify. case_decide; eauto. case_decide; clarify. }
-    sYieldIR "IST" "TID". { case_bool_decide; set_solver. }
+    sYieldIR "IST" "TID".
 
     iApply (wsim_mem_cmp with "E");
       [try prove_inline_cond|try prove_sb_cond|unfold_cris_defs|..]; eauto.
     { instantiate (1:=0%Z). case_bool_decide; clarify; des_ifs; ss. }
     iIntros "_". cStepsT.
-    sYieldIR "IST" "TID". { case_bool_decide; set_solver. }
+    sYieldIR "IST" "TID".
 
     cByCoind CIH. iFrame. done.
   (*SLOW*)Qed.
